prove memory safety for Shift

code/experimental/rsa/Shift.fst
@@ -14,44 +14,57 @@ let bn_tbit = 0x8000000000000000uL
 let bn_mask2 = 0xffffffffffffffffuL
 
 val lshift_loop:
-    a:bignum -> count:U32.t{U32.v count <= length a} -> nw:U32.t ->
-    lb:U32.t -> res:bignum{U32.(v (count +^ nw)) < length res} -> Stack unit
+    a:bignum{length a > 0} ->
+    count:U32.t{U32.v count <= length a} ->
+    nw:U32.t -> lb:U32.t{0 < U32.v lb /\ U32.v lb < 64} ->
+    res:bignum{length res = length a + U32.v nw + 1 /\ U32.v count + U32.v nw < length res /\ disjoint a res} -> 
+    Stack unit
 	(requires (fun h -> live h a /\ live h res))
 	(ensures (fun h0 _ h1 -> live h0 a /\ live h0 res /\ 
         live h1 a /\ live h1 res /\ modifies_1 res h0 h1))
+
 let rec lshift_loop a count nw lb res =
     if U32.(count >^ 0ul) then
-        let count = U32.(count -^ 1ul) in
-        let l = a.(count) in
-        let ind = U32.(nw +^ count +^ 1ul) in
-        let rb = U32.(bn_bits2 -^ lb) in
+        let ind = U32.(nw +^ count) in
         let tmp = res.(ind) in
-        res.(ind) <- U64.(tmp |^ ((l >>^ rb) &^ bn_mask2));
-        res.(U32.(ind -^ 1ul)) <- U64.((l <<^ lb) &^ bn_mask2);
+        let count = U32.(count -^ 1ul) in
+        let t1 = a.(count) in
+        let rb = U32.(64ul -^ lb) in
+        assert(0 < U32.v rb /\ U32.v rb < 64);
+        res.(ind) <- U64.(tmp |^ (U64.(t1 >>^ rb) &^ bn_mask2));
+        res.(U32.(ind -^ 1ul)) <- U64.((t1 <<^ lb) &^ bn_mask2);
         lshift_loop a count nw lb res
     else ()
 
 (* res = a << n *)
 val lshift:
-    aLen:U32.t -> a:bignum{length a = U32.v aLen} -> nCount:U32.t ->
-    res:bignum{length res = U32.(v (aLen +^ (nCount /^ bn_bits2) +^ 1ul))} -> Stack unit
+    aLen:U32.t{U32.v aLen > 0} ->
+    a:bignum{length a = U32.v aLen} -> nCount:U32.t{U32.v nCount> 0} ->
+    res:bignum{length res = U32.v aLen + U32.v nCount / 64 + 1 /\ disjoint a res} -> 
+    Stack unit
 	(requires (fun h -> live h a /\ live h res))
 	(ensures (fun h0 _ h1 -> live h0 a /\ live h0 res /\ 
         live h1 a /\ live h1 res /\ modifies_1 res h0 h1))
+
 let lshift aLen a nCount res =
-    let nw = U32.(nCount/^ bn_bits2) in
+    let nw = U32.(nCount/^ 64ul) in
     let resLen = U32.(aLen +^ nw) in
-    let lb = U32.(nCount %^ bn_bits2) in
-    (if U32.(lb =^ 0ul) then 
+    let lb = U32.(nCount %^ 64ul) in
+    (if U32.(lb =^ 0ul) then
         blit a 0ul res nw aLen
     else lshift_loop a aLen nw lb res)
 
+
 val rshift1_loop:
-    a:bignum -> carry:U64.t -> ind:U32.t{U32.v ind <= length a} ->
-    res:bignum{U32.v ind <= length res} -> Stack unit
+    a:bignum -> 
+    carry:U64.t -> 
+    ind:U32.t{U32.v ind < length a} ->
+    res:bignum{U32.v ind < length res /\ length res = length a} -> 
+    Stack unit
     (requires (fun h -> live h a /\ live h res))
 	(ensures (fun h0 _ h1 -> live h0 a /\ live h0 res /\ 
         live h1 a /\ live h1 res /\ modifies_1 res h0 h1))
+
 let rec rshift1_loop a carry ind res =
     if U32.(ind >^ 0ul) then
         let ind = U32.(ind -^ 1ul) in
@@ -63,13 +76,16 @@ let rec rshift1_loop a carry ind res =
 
 (* res = a >> 1 *)
 val rshift1:
-    aLen:U32.t -> a:bignum{length a = U32.v aLen} ->
-    res:bignum{length res = U32.v aLen /\ length res = U32.(v (aLen -^ 1ul))} -> Stack unit
+    aLen:U32.t{U32.v aLen > 0} ->
+    a:bignum{length a = U32.v aLen} ->
+    res:bignum{length res = U32.v aLen} -> Stack unit
 	(requires (fun h -> live h a /\ live h res))
 	(ensures (fun h0 _ h1 -> live h0 a /\ live h0 res /\ 
         live h1 a /\ live h1 res /\ modifies_1 res h0 h1))
+
+#set-options "--z3rlimit 50"
+
 let rshift1 aLen a res =
-    (* if a = 0 then res = 0 *)
     let i = U32.(aLen -^ 1ul) in
     let tmp = a.(i) in
     let carry = if U64.((tmp &^ 1uL) =^ 1uL) then bn_tbit else 0uL in
